ok

SStructTT/SStruct/Erasure/Normalize.lean
@@ -7,10 +7,57 @@ variable {Srt : Type}
 
 lemma Erased.value_step {m n : Tm Srt} :
     Value m -> m ~>> n -> False := by
-  intro vl st; induction vl generalizing n
-  all_goals cases st <;> aesop
+  intro vl st
+  cases st with
+  | inl st =>
+    induction st
+    all_goals cases vl; try aesop
+  | inr st =>
+    induction st
+    all_goals cases vl; try aesop
+
+@[simp]def drop_count : Tm Srt -> Nat
+  | .var _ => 0
+  | .lam m _ => drop_count m
+  | .app m n => drop_count m + drop_count n
+  | .tup m n _ => drop_count m + drop_count n
+  | .prj m n => drop_count m + drop_count n
+  | .tt => 0
+  | .ff => 0
+  | .ite m n1 n2 => drop_count m + drop_count n1 + drop_count n2
+  | .rw m => drop_count m
+  | .drop m n => 1 + drop_count m + drop_count n
+  | .ptr _ => 0
+  | .null => 0
+
+def DropCount : Tm Srt -> Tm Srt -> Prop  :=
+  InvImage (. < .) drop_count
+
+lemma Step0.sub_drop : Subrelation (flip Step0) (@DropCount Srt) := by
+  intro m m' st; simp[DropCount,InvImage]; induction st
+  all_goals try (solve| aesop)
+
+lemma Step0.flip_wf : WellFounded (flip (@Step0 Srt)) := by
+  apply Subrelation.wf Step0.sub_drop
+  eta_reduce
+  apply InvImage.wf
+  apply Nat.lt_wfRel.wf
+
+theorem Erased.normalize0 {m' : Tm Srt} : SN Step0 m' := by
+  have ⟨h⟩ := @Step0.flip_wf Srt
+  apply SN.ofAcc (h m')
 
 variable [ord : SrtOrder Srt]
+
+theorem Erased.normalize1 {A m : SStruct.Tm Srt} {m'} :
+    [] ;; [] ⊢ m ▷ m' : A -> SN Step1 m' := by
+  intro er
+  have sn := er.toDynamic.normalize
+  induction sn generalizing m'
+  case intro m h ih =>
+  constructor; intro n' st'
+  have ⟨n, st, ern⟩ := er.preservation1 st'
+  apply ih <;> assumption
 
 theorem Erased.normalize {A m : SStruct.Tm Srt} {m'} :
     [] ;; [] ⊢ m ▷ m' : A -> SN Step m' := by
@@ -20,4 +67,55 @@ theorem Erased.normalize {A m : SStruct.Tm Srt} {m'} :
   case intro m h ih =>
   constructor; intro n' st'
   have ⟨n, st, ern⟩ := er.preservation st'
-  apply ih <;> assumption
+  cases st with
+  | inl => aesop
+  | inr =>
+    subst_vars
+    apply ih <;> try assumption
+    sorry
+
+-- theorem Erased.normalize {A m : SStruct.Tm Srt} {m'} :
+--     [] ;; [] ⊢ m ▷ m' : A -> SN Step m' := by
+--   intro er; unfold Step
+--   apply Classical.byContradiction; intro nn
+--   have := SN.negate nn
+--   constructor
+
+-- theorem Erased.normalize0 {m' : Tm Srt} : SN Step0 m' := by
+--   induction m'
+--   sorry
+--   sorry
+--   case app ihm ihn =>
+--     replace ⟨ihm⟩ := ihm
+--     replace ⟨ihn⟩ := ihn
+--     constructor
+--     apply Classical.byContradiction
+--     intro h; simp at h
+--     have ⟨x, st, nn⟩ := h
+--     cases st
+--     case a.h.app_M =>
+
+--       sorry
+--     case a.h.app_N =>
+--       sorry
+
+
+--     sorry
+
+
+  -- constructor
+  -- apply Classical.byContradiction; intro h
+  -- simp at h
+  -- induction m'
+  -- case a.h.var =>
+  --   have ⟨m, st, sn⟩ := h
+  --   cases st
+  -- case a.h.lam =>
+  --   have ⟨m, st, sn⟩ := h
+  --   cases st
+  -- case a.h.app ihm ihn =>
+  --   have ⟨m, st, sn⟩ := h
+  --   cases st
+  --   case app_M x st =>
+  --     sorry
+  --   case app_N => sorry
